semantics/semBakeryScript.sml
@@ -476,4 +476,53 @@ Proof
   metis_tac [trans_s_submap_gen]
 QED
 
+val free_variables_def = Define `
+  (free_variables (Nil) = {}) /\
+  (free_variables (IfThen v p c1 c2) = {(v,p)} ∪ (free_variables c1 ∪ free_variables c2)) /\
+  (free_variables (Com p1 v1 p2 v2 c) = {(v1,p1)} ∪ (free_variables c DELETE (v2,p2))) /\
+  (free_variables (Let v p f vl c) = set(MAP (λv. (v,p)) vl) ∪ (free_variables c DELETE (v,p))) /\
+  (free_variables (Sel p b q c) = free_variables c)
+`
+
+val defined_vars_def = Define `
+  defined_vars (s,c) = FDOM s`
+
+val no_undefined_vars_def = Define `
+  no_undefined_vars (s,c) = (free_variables c ⊆ FDOM s)`
+
+Theorem defined_vars_mono:
+  ∀sc alpha sc'. trans sc alpha sc' ⇒ defined_vars sc ⊆ defined_vars sc'
+Proof
+  ho_match_mp_tac trans_ind
+  >> rpt strip_tac
+  >> fs[defined_vars_def,SUBSET_OF_INSERT]
+QED
+
+Theorem free_vars_mono:
+  ∀sc alpha sc'. trans sc alpha sc'
+    ⇒ (free_variables(SND sc') DIFF defined_vars sc' ⊆ free_variables(SND sc) DIFF defined_vars sc)
+Proof
+  ho_match_mp_tac (theorem "trans_strongind")
+  >> rpt strip_tac
+  >> imp_res_tac defined_vars_mono
+  >> fs[free_variables_def,defined_vars_def,DIFF_INSERT] >> rw[]
+  >> fs[DELETE_DEF,DIFF_DEF,SUBSET_DEF] >> rpt strip_tac
+  >> fs[] >> metis_tac[]
+QED
+
+Theorem no_undefined_vars_trans_pres:
+  ∀sc alpha sc'. no_undefined_vars sc ∧ trans sc alpha sc' ⇒ no_undefined_vars sc'
+Proof
+  rpt gen_tac >> disch_then(MAP_EVERY assume_tac o CONJUNCTS)
+  >> qpat_x_assum `no_undefined_vars _` mp_tac
+  >> qpat_x_assum `trans _ _ _` mp_tac
+  >> MAP_EVERY (W(curry Q.SPEC_TAC)) (rev [`sc`,`alpha`,`sc'`])
+  >> ho_match_mp_tac (theorem "trans_strongind")
+  >> rpt strip_tac
+  >> imp_res_tac defined_vars_mono
+  >> imp_res_tac free_vars_mono
+  >> fs[no_undefined_vars_def,free_variables_def,DELETE_SUBSET_INSERT,defined_vars_def,SUBSET_OF_INSERT]
+  >> fs[SUBSET_DEF,INSERT_DEF,DIFF_DEF] >> metis_tac[]
+QED
+
 val _ = export_theory ()
